WIP CBOR.Spec.Raw.Format

src/lowparse/LowParse.Spec.Recursive.fst
@@ -6,7 +6,7 @@ module Seq = FStar.Seq
 
 let parse_recursive_aux_ext
   (p: parse_recursive_param)
-  (ih1 ih2: parser (parse_recursive_kind p.parse_header_kind) p.t)
+  (ih1 ih2: tot_parser (parse_recursive_kind p.parse_header_kind) p.t)
   (b: bytes)
   (prf: (
     (b': bytes { Seq.length b' < Seq.length b }) -> // IMPORTANT: lt, not leq, to make induction work
@@ -16,18 +16,20 @@ let parse_recursive_aux_ext
 : Lemma
   (parse (parse_recursive_aux p ih1) b == parse (parse_recursive_aux p ih2) b)
 = p.synth_inj;
-  parse_synth_eq (parse_recursive_alt p ih1) p.synth_ b;
-  parse_synth_eq (parse_recursive_alt p ih2) p.synth_ b;
-  parse_dtuple2_eq p.parse_header (parse_recursive_payload p ih1) b;
-  parse_dtuple2_eq p.parse_header (parse_recursive_payload p ih2) b;
+  tot_parse_synth_eq (parse_recursive_alt p ih1) p.synth_ b;
+  tot_parse_synth_eq (parse_recursive_alt p ih2) p.synth_ b;
   match parse p.parse_header b with
   | None -> ()
   | Some (h, consumed) ->
     parser_kind_prop_equiv p.parse_header_kind p.parse_header;
     let b' = Seq.slice b consumed (Seq.length b) in
+    tot_parse_nlist_parse_nlist (p.count h) ih1 b';
+    tot_parse_nlist_parse_nlist (p.count h) ih2 b';
     parse_nlist_ext
       (p.count h)
+      #(parse_recursive_kind p.parse_header_kind)
       ih1
+      #(parse_recursive_kind p.parse_header_kind)
       ih2
       b'
       (fun b'' -> prf b'')
@@ -35,9 +37,9 @@ let parse_recursive_aux_ext
 let rec parse_recursive_step
   (p: parse_recursive_param)
   (n: nat)
-: Tot (parser (parse_recursive_kind p.parse_header_kind) p.t)
+: Tot (tot_parser (parse_recursive_kind p.parse_header_kind) p.t)
 = if n = 0
-  then fail_parser _ _
+  then tot_fail_parser _ _
   else parse_recursive_aux p (parse_recursive_step p (n - 1))
 
 let closure
@@ -71,21 +73,22 @@ let parse_recursive_step_ext
 = parse_recursive_step_ext_gen p (closure input) fuel input
 
 let parse_recursive
-  (p: parse_recursive_param)
-: Tot (parser (parse_recursive_kind p.parse_header_kind) p.t)
-= close_by_fuel (parse_recursive_step p) closure (parse_recursive_step_ext p)
+  p
+= magic () // close_by_fuel (parse_recursive_step p) closure (parse_recursive_step_ext p)
 
 let parse_recursive_eq
   (p: parse_recursive_param)
   (b: bytes)
 : Lemma
   (parse (parse_recursive p) b == parse (parse_recursive_aux p (parse_recursive p)) b)
-= let c = closure b in
+= admit () (*
+  let c = closure b in
   let q = parse_recursive_step p (c - 1) in
   assert (parse (parse_recursive p) b == parse (parse_recursive_aux p q) b);
   parse_recursive_aux_ext p q (parse_recursive p) b (fun input' -> // here hypothesis Seq.length input' < Seq.length input is used
     parse_recursive_step_ext p (c - 1) input'
   )
+*)
 
 let has_pred_level
   (#p: parse_recursive_param)
@@ -108,67 +111,73 @@ let mk_serialize_recursive_with_level
   (#pp: parse_recursive_param)
   (#sp: serialize_recursive_param pp)
   (n: nat)
-  (s: serializer (parse_filter (parse_recursive_alt pp (parse_recursive pp)) (has_pred_level sp n)))
-: Tot (serializer (parse_filter (parse_recursive pp) (has_level sp.level n)))
+  (s: tot_serializer #(parse_filter_kind (and_then_kind pp.parse_header_kind parse_recursive_payload_kind)) (tot_parse_filter (parse_recursive_alt pp (parse_recursive pp)) (has_pred_level sp n)))
+: Tot (tot_serializer #(parse_filter_kind (parse_recursive_kind pp.parse_header_kind)) (tot_parse_filter (parse_recursive pp) (has_level sp.level n)))
 = let s'
     (x: parse_filter_refine (has_level sp.level n))
-  : GTot bytes
+  : Tot bytes
   = level_correct' sp n x;
     s (sp.synth_recip x)
   in
-  mk_serializer
+  mk_tot_serializer
     _
     s'
     (fun x ->
       let b = s' x in
       level_correct' sp n x;
-      parse_filter_eq (parse_recursive_alt pp (parse_recursive pp)) (has_pred_level sp n) b;
-      parse_filter_eq (parse_recursive pp) (has_level sp.level n) b;
+      tot_parse_filter_eq (parse_recursive_alt pp (parse_recursive pp)) (has_pred_level sp n) b;
+      tot_parse_filter_eq (parse_recursive pp) (has_level sp.level n) b;
       parse_recursive_eq pp b;
       pp.synth_inj;
-      parse_synth_eq (parse_recursive_alt pp (parse_recursive pp)) pp.synth_ b
+      tot_parse_synth_eq (parse_recursive_alt pp (parse_recursive pp)) pp.synth_ b
     )
+
+#push-options "--z3rlimit 128 --print_implicits --ifuel 8"
+#restart-solver
 
 let mk_serialize_recursive_alt_with_level
   (#pp: parse_recursive_param)
   (#sp: serialize_recursive_param pp)
   (n: nat)
-  (s: ((l: pp.header) -> serializer (weaken parse_recursive_payload_kind (parse_nlist (pp.count l) (parse_recursive pp) `parse_filter` list_has_pred_level sp.level n))))
-: Tot (serializer (parse_filter (parse_recursive_alt pp (parse_recursive pp)) (has_pred_level sp n)))
-= let s1 = serialize_dtuple2 sp.serialize_header s in
+  (s: ((l: pp.header) -> tot_serializer #parse_recursive_payload_kind (tot_weaken parse_recursive_payload_kind (tot_parse_nlist (pp.count l) (parse_recursive pp) `tot_parse_filter` list_has_pred_level sp.level n))))
+: Tot (tot_serializer #(parse_filter_kind (and_then_kind pp.parse_header_kind parse_recursive_payload_kind)) #(parse_filter_refine #(parse_recursive_alt_t pp.t pp.header pp.count) (has_pred_level #pp sp n)) (tot_parse_filter #_ #(parse_recursive_alt_t pp.t pp.header pp.count) (parse_recursive_alt pp (parse_recursive pp)) (has_pred_level sp n)))
+= let s1 = tot_serialize_dtuple2 sp.serialize_header s in
   let s'
     (x: parse_filter_refine (has_pred_level sp n))
   = let (| l, c |) = x in
     s1 (| l, c |)
   in
-  mk_serializer
-    _
+  mk_tot_serializer
+    #(parse_filter_kind (and_then_kind pp.parse_header_kind parse_recursive_payload_kind))
+    #(parse_filter_refine #(parse_recursive_alt_t pp.t pp.header pp.count) (has_pred_level #pp sp n)) (tot_parse_filter #_ #(parse_recursive_alt_t pp.t pp.header pp.count) (parse_recursive_alt pp (parse_recursive pp)) (has_pred_level sp n))
     s'
     (fun x ->
       let b = s' x in
-      parse_filter_eq (parse_recursive_alt pp (parse_recursive pp)) (has_pred_level sp n) b;
-      parse_dtuple2_eq pp.parse_header (parse_recursive_payload pp (parse_recursive pp)) b;
-      parse_dtuple2_eq pp.parse_header (fun l -> weaken parse_recursive_payload_kind (parse_nlist (pp.count l) (parse_recursive pp) `parse_filter` list_has_pred_level sp.level n)) b;
+      tot_parse_filter_eq (parse_recursive_alt pp (parse_recursive pp)) (has_pred_level sp n) b;
+      assume False (*
       let Some (l, consumed) = parse pp.parse_header b in
       let b' = Seq.slice b consumed (Seq.length b) in
-      parse_filter_eq (parse_nlist (pp.count l) (parse_recursive pp)) (list_has_pred_level sp.level n) b'
+      tot_parse_filter_eq (tot_parse_nlist (pp.count l) (parse_recursive pp)) (list_has_pred_level sp.level n) b'
+*)      
     )
+
+(* WIP
 
 let serialize_recursive_list_has_pred_level_zero
   (#pp: parse_recursive_param)
   (sp: serialize_recursive_param pp)
   (n: nat { n == 0 })
   (len: nat)
-: serializer (parse_nlist len (parse_recursive pp) `parse_filter` list_has_pred_level sp.level n)
-= let s' : bare_serializer (parse_filter_refine #(nlist len pp.t) (list_has_pred_level sp.level n)) = fun _ -> Seq.empty in
-  mk_serializer
+: tot_serializer (tot_parse_nlist len (parse_recursive pp) `tot_parse_filter` list_has_pred_level sp.level n)
+= let s' : tot_bare_serializer (parse_filter_refine #(nlist len pp.t) (list_has_pred_level sp.level n)) = fun _ -> Seq.empty in
+  mk_tot_serializer
     _
     s'
     (fun x ->
       assert (Nil? x);
       let res : bytes = Seq.empty in
-      parse_filter_eq (parse_nlist len (parse_recursive pp)) (list_has_pred_level sp.level n) res;
-      parse_nlist_eq n (parse_recursive pp) res
+      tot_parse_filter_eq (tot_parse_nlist len (parse_recursive pp)) (list_has_pred_level sp.level n) res;
+      tot_parse_nlist_eq n (parse_recursive pp) res
     )
 
 #restart-solver
@@ -230,12 +239,12 @@ let rec serialize_recursive_with_level
         )
       )
     )
+*)
 
 let serialize_recursive
-  (#pp: parse_recursive_param)
-  (sp: serialize_recursive_param pp)
-: Tot (serializer (parse_recursive pp))
-=
+  #pp sp
+= admit ()
+(*
   let s' (x: pp.t) : GTot bytes =
     serialize_recursive_with_level sp (sp.level x) x
   in
@@ -245,14 +254,12 @@ let serialize_recursive
     (fun x ->
       parse_filter_eq (parse_recursive pp) (has_level sp.level (sp.level x)) (s' x)
     )
+*)
 
 let serialize_recursive_eq
-  (#pp: parse_recursive_param)
-  (sp: serialize_recursive_param pp)
-  (x: pp.t)
-: Lemma
-  (serialize (serialize_recursive sp) x == serialize (serialize_recursive_aux sp) x)
-=
+  #pp sp x
+= admit () (*
   Classical.forall_intro (parse_recursive_eq pp);
   let s' = serialize_ext (parse_recursive pp) (serialize_recursive sp) (parse_recursive_aux pp (parse_recursive pp)) in
   serializer_unique _ (serialize_recursive_aux sp) s' x
+*)
